More Boogie DSL, more proof experiments

LeanBoogie/Boog.lean
@@ -3,25 +3,52 @@ open Std (HashSet HashMap)
 
 namespace Boog
 
+-- Lean-auto is able to reason about strings just fine:
+-- example : "a" ++ "b" = "ab" := by auto
+
 -- # Boogie state monad
 
-structure BoogieState where
-  vars : Std.HashMap String Int
-deriving Inhabited
+-- structure BoogieState where
+  -- vars : Std.HashMap String Int
+abbrev BoogieState := String -> Int
+-- deriving Inhabited
 
 abbrev Boog : Type -> Type := StateM BoogieState
 
 def Boog.skip : Boog Unit := pure ()
 def Boog.seq (a b : Boog Unit) : Boog Unit := do a; b
 
+-- def update [DecidableEq A] (f : A -> B) (a : A) (b : B) : A -> B :=
+--   fun x => if x = a then b else f x
+def update (a : String) (b : Int) : (String -> Int) -> (String -> Int) :=
+  fun f x => if x = a then b else f x
+
 def Boog.set (v : String) (e : Boog Int) : Boog Unit := do
   let val <- e
-  modifyThe BoogieState (fun s => { s with vars := s.vars.insert v val })
+  -- modifyThe BoogieState (fun s => { s with vars := s.vars.insert v val })
+  modifyThe BoogieState
+      (fun f x => if x = v then val else f x)
+    -- (update v val)
 
 def Boog.get (v : String) : Boog Int := do
-  return (<- getThe BoogieState).vars.getD v 0
+  let state <- getThe BoogieState
+  return state v
+  -- return (<- getThe BoogieState).vars.getD v 0
 
 def Boog.ifthen (c : Boog Bool) (t : Boog Unit) : Boog Unit := do
   if <- c then t
+
 def Boog.ifthenelse (c : Boog Bool) (t e : Boog Unit) : Boog Unit := do
   if <- c then t else e
+
+-- # Using HashMap instead...
+
+-- Lean-auto doesn't deal well with this:
+-- example (m : Std.HashMap String Int) :
+--     (m.insert "a" 1).insert "a" 0
+--   = (m.insert "a" 2).insert "a" 0
+--   := by auto
+--
+-- But we can provide lemmas like these:
+-- theorem HashMap.lww (m : Std.HashMap String B) : (m.insert a val1).insert a val2 = m.insert a val2 := by
+--   sorry
